pcuic/theories/PCUICAstUtils.v
@@ -43,102 +43,6 @@ Fixpoint string_of_term (t : term) :=
   end.
 Local Close Scope string_scope.
 
-(** Make a lambda/let-in string of abstractions from a context [Γ], ending with term [t]. *)
-
-Definition mkLambda_or_LetIn d t :=
-  match d.(decl_body) with
-  | None => tLambda d.(decl_name) d.(decl_type) t
-  | Some b => tLetIn d.(decl_name) b d.(decl_type) t
-  end.
-
-Definition it_mkLambda_or_LetIn (l : context) (t : term) :=
-  List.fold_left (fun acc d => mkLambda_or_LetIn d acc) l t.
-
-(** Make a prod/let-in string of abstractions from a context [Γ], ending with term [t]. *)
-
-Definition mkProd_or_LetIn d t :=
-  match d.(decl_body) with
-  | None => tProd d.(decl_name) d.(decl_type) t
-  | Some b => tLetIn d.(decl_name) b d.(decl_type) t
-  end.
-
-Definition it_mkProd_or_LetIn (l : context) (t : term) :=
-  List.fold_left (fun acc d => mkProd_or_LetIn d acc) l t.
-
-Definition map_decl f (d : context_decl) :=
-  {| decl_name := d.(decl_name);
-     decl_body := option_map f d.(decl_body);
-     decl_type := f d.(decl_type) |}.
-
-Lemma map_decl_type f decl : f (decl_type decl) = decl_type (map_decl f decl).
-Proof. destruct decl; reflexivity. Qed.
-
-Lemma map_decl_body f decl : option_map f (decl_body decl) = decl_body (map_decl f decl).
-Proof. destruct decl; reflexivity. Qed.
-
-Lemma option_map_decl_body_map_decl f x :
-  option_map decl_body (option_map (map_decl f) x) =
-  option_map (option_map f) (option_map decl_body x).
-Proof. destruct x; reflexivity. Qed.
-
-Lemma option_map_decl_type_map_decl f x :
-  option_map decl_type (option_map (map_decl f) x) =
-  option_map f (option_map decl_type x).
-Proof. destruct x; reflexivity. Qed.
-
-Definition map_context f c :=
-  List.map (map_decl f) c.
-
-Definition map_constant_body f decl :=
-  {| cst_type := f decl.(cst_type);
-     cst_body := option_map f decl.(cst_body);
-     cst_universes := decl.(cst_universes) |}.
-
-Lemma map_cst_type f decl : f (cst_type decl) = cst_type (map_constant_body f decl).
-Proof. destruct decl; reflexivity. Qed.
-
-Lemma map_cst_body f decl : option_map f (cst_body decl) = cst_body (map_constant_body f decl).
-Proof. destruct decl; reflexivity. Qed.
-
-Definition map_def {A B} (tyf bodyf : A -> B) (d : def A) :=
-  {| dname := d.(dname); dtype := tyf d.(dtype); dbody := bodyf d.(dbody); rarg := d.(rarg) |}.
-
-Lemma map_dtype {A B} (f : A -> B) (g : A -> B) (d : def A) :
-  f (dtype d) = dtype (map_def f g d).
-Proof. destruct d; reflexivity. Qed.
-
-Lemma map_dbody {A B} (f : A -> B) (g : A -> B) (d : def A) :
-  g (dbody d) = dbody (map_def f g d).
-Proof. destruct d; reflexivity. Qed.
-
-Definition app_context (Γ Γ' : context) : context := (Γ' ++ Γ)%list.
-Notation " Γ  ,,, Γ' " := (app_context Γ Γ') (at level 25, Γ' at next level, left associativity) : pcuic.
-
-Lemma app_context_assoc Γ Γ' Γ'' : Γ ,,, (Γ' ,,, Γ'') = Γ ,,, Γ' ,,, Γ''.
-Proof. unfold app_context; now rewrite app_assoc. Qed.
-
-Lemma app_context_cons Γ Γ' A : Γ ,,, (Γ' ,, A) = (Γ ,,, Γ') ,, A.
-Proof.
-  now rewrite (app_context_assoc _ _ [A]).
-Qed.
-
-Lemma app_context_length Γ Γ' : #|Γ ,,, Γ'| = #|Γ'| + #|Γ|.
-Proof. unfold app_context. now rewrite app_length. Qed.
-
-Lemma nth_error_app_context_ge v Γ Γ' : #|Γ'| <= v -> nth_error (Γ ,,, Γ') v = nth_error Γ (v - #|Γ'|).
-Proof. apply nth_error_app_ge. Qed.
-
-Lemma nth_error_app_context_lt v Γ Γ' : v < #|Γ'| -> nth_error (Γ ,,, Γ') v = nth_error Γ' v.
-Proof. apply nth_error_app_lt. Qed.
-
-Lemma app_context_nil_l Γ : [] ,,, Γ = Γ.
-Proof. unfold app_context; now rewrite app_nil_r. Qed.
-
-Lemma map_app_context f Γ Γ' : map f (Γ ,,, Γ') = map f Γ ,,, map f Γ'.
-Proof.
-  induction Γ'; simpl; congruence.
-Qed.
-
 Fixpoint decompose_app_rec (t : term) l :=
   match t with
   | tApp f a => decompose_app_rec f (a :: l)
@@ -176,12 +80,6 @@ Fixpoint decompose_prod (t : term) : (list name) * (list term) * term :=
   | _ => ([], [], t)
   end.
 
-Definition get_ident (n : name) : string :=
-  match n with
-  | nAnon => "XX"
-  | nNamed i => i
-  end.
-
 Fixpoint remove_arity (n : nat) (t : term) : term :=
   match n with
   | O => t
@@ -196,14 +94,6 @@ Definition isConstruct_app t :=
   | tConstruct _ _ _ => true
   | _ => false
   end.
-
-Fixpoint lookup_mind_decl (id : ident) (decls : global_env)
- := match decls with
-    | nil => None
-    | (kn, InductiveDecl d) :: tl =>
-      if ident_eq kn id then Some d else lookup_mind_decl id tl
-    | _ :: tl => lookup_mind_decl id tl
-    end.
 
 (* was mind_decl_to_entry *)
 Definition mind_body_to_entry (decl : mutual_inductive_body)
@@ -239,12 +129,6 @@ Proof.
                                                 (snd (fst x))) ind_ctors).
 Defined.
 
-Definition arities_context (l : list one_inductive_body) :=
-  rev_map (fun ind => vass (nNamed ind.(ind_name)) ind.(ind_type)) l.
-
-Lemma arities_context_length l : #|arities_context l| = #|l|.
-Proof. unfold arities_context. now rewrite rev_map_length. Qed.
-
 Fixpoint decompose_prod_assum (Γ : context) (t : term) : context * term :=
   match t with
   | tProd n A B => decompose_prod_assum (Γ ,, vass n A) B
@@ -263,10 +147,7 @@ Fixpoint decompose_prod_n_assum (Γ : context) n (t : term) : option (context * 
     end
   end.
 
-Lemma it_mkProd_or_LetIn_app l l' t :
-  it_mkProd_or_LetIn (l ++ l') t = it_mkProd_or_LetIn l' (it_mkProd_or_LetIn l t).
-Proof. induction l in l', t |- *; simpl; auto. Qed.
-
+(* todo move *)
 Lemma it_mkLambda_or_LetIn_app l l' t :
   it_mkLambda_or_LetIn (l ++ l') t = it_mkLambda_or_LetIn l' (it_mkLambda_or_LetIn l t).
 Proof. induction l in l', t |- *; simpl; auto. Qed.
@@ -303,342 +184,9 @@ Proof.
   case: x => [na [body|] ty'] /=; by rewrite IHctx' // /snoc -app_assoc.
 Qed.
 
-Fixpoint reln (l : list term) (p : nat) (Γ0 : list context_decl) {struct Γ0} : list term :=
-  match Γ0 with
-  | [] => l
-  | {| decl_body := Some _ |} :: hyps => reln l (p + 1) hyps
-  | {| decl_body := None |} :: hyps => reln (tRel p :: l) (p + 1) hyps
-  end.
-
-Definition to_extended_list_k Γ k := reln [] k Γ.
-Definition to_extended_list Γ := to_extended_list_k Γ 0.
-
-Lemma reln_list_lift_above l p Γ :
-  Forall (fun x => exists n, x = tRel n /\ p <= n /\ n < p + length Γ) l ->
-  Forall (fun x => exists n, x = tRel n /\ p <= n /\ n < p + length Γ) (reln l p Γ).
-Proof.
-  generalize (le_refl p).
-  generalize p at 1 3 5.
-  induction Γ in p, l |- *. simpl. auto.
-  intros. destruct a. destruct decl_body. simpl.
-  assert(p0 <= S p) by lia.
-  specialize (IHΓ l (S p) p0 H1). rewrite <- Nat.add_succ_comm, Nat.add_1_r.
-  simpl in *. rewrite <- Nat.add_succ_comm in H0. eauto.
-  simpl in *.
-  specialize (IHΓ (tRel p :: l) (S p) p0 ltac:(lia)). rewrite <- Nat.add_succ_comm, Nat.add_1_r.
-  eapply IHΓ. simpl in *. rewrite <- Nat.add_succ_comm in H0. auto.
-  simpl in *.
-  constructor. exists p. intuition lia. auto.
-Qed.
-
-Lemma to_extended_list_k_spec Γ k :
-  Forall (fun x => exists n, x = tRel n /\ k <= n /\ n < k + length Γ) (to_extended_list_k Γ k).
-Proof.
-  pose (reln_list_lift_above [] k Γ).
-  unfold to_extended_list_k.
-  forward f. constructor. apply f.
-Qed.
-
-Lemma to_extended_list_lift_above Γ :
-  Forall (fun x => exists n, x = tRel n /\ n < length Γ) (to_extended_list Γ).
-Proof.
-  pose (reln_list_lift_above [] 0 Γ).
-  unfold to_extended_list.
-  forward f. constructor. eapply Forall_impl; eauto. intros.
-  destruct H; eexists; intuition eauto.
-Qed.
-
-Fixpoint reln_alt p Γ :=
-  match Γ with
-  | [] => []
-  | {| decl_body := Some _ |} :: Γ => reln_alt (p + 1) Γ
-  | {| decl_body := None |} :: Γ => tRel p :: reln_alt (p + 1) Γ
-  end.
-
-Lemma reln_alt_eq l Γ k : reln l k Γ = List.rev (reln_alt k Γ) ++ l.
-Proof.
-  induction Γ in l, k |- *; simpl; auto.
-  destruct a as [na [body|] ty]; simpl.
-  now rewrite IHΓ.
-  now rewrite IHΓ -app_assoc.
-Qed.
-
-Lemma to_extended_list_k_cons d Γ k :
-  to_extended_list_k (d :: Γ) k =
-  match d.(decl_body) with
-  | None => to_extended_list_k Γ (S k) ++ [tRel k]
-  | Some b => to_extended_list_k Γ (S k)
-  end.
-Proof.
-  rewrite /to_extended_list_k reln_alt_eq. simpl.
-  destruct d as [na [body|] ty]. simpl.
-  now rewrite reln_alt_eq Nat.add_1_r.
-  simpl. rewrite reln_alt_eq.
-  now rewrite -app_assoc !app_nil_r Nat.add_1_r.
-Qed.
-
-Fixpoint context_assumptions (Γ : context) :=
-  match Γ with
-  | [] => 0
-  | d :: Γ =>
-    match d.(decl_body) with
-    | Some _ => context_assumptions Γ
-    | None => S (context_assumptions Γ)
-    end
-  end.
-
-Definition map_one_inductive_body npars arities f (n : nat) m :=
-  match m with
-  | Build_one_inductive_body ind_name ind_type ind_kelim ind_ctors ind_projs =>
-    Build_one_inductive_body ind_name
-                             (f 0 ind_type)
-                             ind_kelim
-                             (map (on_pi2 (f arities)) ind_ctors)
-                             (map (on_snd (f (S npars))) ind_projs)
-  end.
-
-Definition fold_context f (Γ : context) : context :=
-  List.rev (mapi (fun k' decl => map_decl (f k') decl) (List.rev Γ)).
-
-Lemma fold_context_alt f Γ :
-  fold_context f Γ =
-  mapi (fun k' d => map_decl (f (Nat.pred (length Γ) - k')) d) Γ.
-Proof.
-  unfold fold_context. rewrite rev_mapi. rewrite List.rev_involutive.
-  apply mapi_ext. intros. f_equal. now rewrite List.rev_length.
-Qed.
-
-Lemma fold_context_length f Γ : length (fold_context f Γ) = length Γ.
-Proof.
-  unfold fold_context. now rewrite !List.rev_length mapi_length List.rev_length.
-Qed.
-
-Lemma fold_context_snoc0 f Γ d : fold_context f (d :: Γ) = fold_context f Γ ,, map_decl (f (length Γ)) d.
-Proof.
-  unfold fold_context.
-  rewrite !rev_mapi !rev_involutive. unfold mapi; rewrite mapi_rec_eqn.
-  unfold snoc. f_equal. now rewrite Nat.sub_0_r List.rev_length.
-  rewrite mapi_rec_Sk. simpl. apply mapi_rec_ext. intros.
-  rewrite app_length !List.rev_length. simpl. f_equal. f_equal. lia.
-Qed.
-
-Lemma fold_context_app f Γ Δ :
-  fold_context f (Δ ++ Γ) = fold_context (fun k => f (length Γ + k)) Δ ++ fold_context f Γ.
-Proof.
-  unfold fold_context.
-  rewrite List.rev_app_distr.
-  rewrite mapi_app. rewrite <- List.rev_app_distr. f_equal. f_equal.
-  apply mapi_ext. intros. f_equal. rewrite List.rev_length. f_equal.
-Qed.
-
-Lemma context_assumptions_fold Γ f : context_assumptions (fold_context f Γ) = context_assumptions Γ.
-Proof.
-  rewrite fold_context_alt.
-  unfold mapi. generalize 0 (Nat.pred #|Γ|).
-  induction Γ as [|[na [body|] ty] tl]; cbn; intros; eauto.
-Qed.
-
-Lemma nth_error_fold_context (f : nat -> term -> term):
-  forall (Γ' Γ'' : context) (v : nat),
-    v < length Γ' -> forall nth,
-    nth_error Γ' v = Some nth ->
-    nth_error (fold_context f Γ') v = Some (map_decl (f (length Γ' - S v)) nth).
-Proof.
-  induction Γ'; intros.
-  - easy.
-  - simpl. destruct v; rewrite fold_context_snoc0.
-    + simpl. repeat f_equal; try lia. simpl in *. congruence.
-    + simpl. apply IHΓ'; simpl in *; (lia || congruence).
-Qed.
-
-Lemma nth_error_fold_context_eq:
-  forall (Γ' : context) (v : nat) f,
-    nth_error (fold_context f Γ') v =
-    option_map (map_decl (f (length Γ' - S v))) (nth_error Γ' v).
-Proof.
-  induction Γ'; intros.
-  - simpl. unfold fold_context, fold_context; simpl. now rewrite nth_error_nil.
-  - simpl. destruct v; rewrite fold_context_snoc0.
-    + simpl. repeat f_equal; try lia.
-    + simpl. apply IHΓ'; simpl in *; (lia || congruence).
-Qed.
-
-Lemma nth_error_ge {Γ Γ' v Γ''} f : length Γ' <= v ->
-  nth_error (Γ' ++ Γ) v =
-  nth_error (fold_context (f 0) Γ' ++ Γ'' ++ Γ) (length Γ'' + v).
-Proof.
-  intros Hv.
-  rewrite -> !nth_error_app_ge, ?fold_context_length. f_equal. lia.
-  rewrite fold_context_length. lia.
-  rewrite fold_context_length. lia. auto.
-Qed.
-
-Lemma nth_error_lt {Γ Γ' Γ'' v} (f : nat -> term -> term) : v < length Γ' ->
-  nth_error (fold_context f Γ' ++ Γ'' ++ Γ) v =
-  option_map (map_decl (f (length Γ' - S v))) (nth_error (Γ' ++ Γ) v).
-Proof.
-  simpl. intros Hv.
-  rewrite -> !nth_error_app_lt.
-  rewrite nth_error_fold_context_eq.
-  do 2 f_equal. lia. now rewrite fold_context_length.
-Qed.
-
-Definition map_mutual_inductive_body f m :=
-  match m with
-  | Build_mutual_inductive_body finite ind_npars ind_pars ind_bodies
-    ind_universes ind_variance =>
-    let arities := arities_context ind_bodies in
-    let pars := fold_context f ind_pars in
-    Build_mutual_inductive_body finite ind_npars pars
-      (mapi (map_one_inductive_body (context_assumptions pars) (length arities) f) ind_bodies)
-      ind_universes ind_variance
-  end.
-
-Lemma ind_type_map f npars_ass arities n oib :
-  ind_type (map_one_inductive_body npars_ass arities f n oib) = f 0 (ind_type oib).
-Proof. destruct oib. reflexivity. Qed.
-
-Lemma ind_ctors_map f npars_ass arities n oib :
-  ind_ctors (map_one_inductive_body npars_ass arities f n oib) =
-  map (on_pi2 (f arities)) (ind_ctors oib).
-Proof. destruct oib; simpl; reflexivity. Qed.
-
-Lemma ind_pars_map f m :
-  ind_params (map_mutual_inductive_body f m) =
-  fold_context f (ind_params m).
-Proof. destruct m; simpl; reflexivity. Qed.
-
-Lemma ind_projs_map f npars_ass arities n oib :
-  ind_projs (map_one_inductive_body npars_ass arities f n oib) =
-  map (on_snd (f (S npars_ass))) (ind_projs oib).
-Proof. destruct oib; simpl. reflexivity. Qed.
-
-Definition test_def {A} (tyf bodyf : A -> bool) (d : def A) :=
-  tyf d.(dtype) && bodyf d.(dbody).
-
-Definition tCaseBrsProp {A} (P : A -> Type) (l : list (nat * A)) :=
-  All (fun x => P (snd x)) l.
-
-Definition tFixProp {A} (P P' : A -> Type) (m : mfixpoint A) :=
-  All (fun x : def A => P x.(dtype) * P' x.(dbody))%type m.
-
-
-Ltac merge_All :=
-  unfold tFixProp, tCaseBrsProp in *;
-  repeat toAll.
-
-
-Lemma map_def_map_def {A B C} (f f' : B -> C) (g g' : A -> B) (d : def A) :
-  map_def f f' (map_def g g' d) = map_def (fun x => f (g x)) (fun x => f' (g' x)) d.
-Proof.
-  destruct d; reflexivity.
-Qed.
-
-Lemma compose_map_def {A B C} (f f' : B -> C) (g g' : A -> B) :
-  compose (A:=def A) (map_def f f') (map_def g g') = map_def (compose f g) (compose f' g').
-Proof. reflexivity. Qed.
-
-Lemma map_def_id {t} x : map_def (@id t) (@id t) x = x.
-Proof. now destruct x. Qed.
 Hint Rewrite @map_def_id @map_id : map.
 
-Lemma map_def_spec {A B} (P P' : A -> Type) (f f' g g' : A -> B) (x : def A) :
-  P' x.(dbody) -> P x.(dtype) -> (forall x, P x -> f x = g x) ->
-  (forall x, P' x -> f' x = g' x) ->
-  map_def f f' x = map_def g g' x.
-Proof.
-  intros. destruct x. unfold map_def. simpl.
-  rewrite !H // !H0 //.
-Qed.
-
-Lemma case_brs_map_spec {A B} {P : A -> Type} {l} {f g : A -> B} :
-  tCaseBrsProp P l -> (forall x, P x -> f x = g x) ->
-  map (on_snd f) l = map (on_snd g) l.
-Proof.
-  intros. red in X.
-  eapply All_map_eq. eapply All_impl; eauto. simpl; intros.
-  apply on_snd_eq_spec; eauto.
-Qed.
-
-Lemma tfix_map_spec {A B} {P P' : A -> Type} {l} {f f' g g' : A -> B} :
-  tFixProp P P' l -> (forall x, P x -> f x = g x) ->
-  (forall x, P' x -> f' x = g' x) ->
-  map (map_def f f') l = map (map_def g g') l.
-Proof.
-  intros.
-  eapply All_map_eq. red in X. eapply All_impl; eauto. simpl.
-  intros. destruct X0;
-  eapply map_def_spec; eauto.
-Qed.
-
-
-Lemma map_def_test_spec {A B}
-      (P P' : A -> Type) (p p' : pred A) (f f' g g' : A -> B) (x : def A) :
-  P x.(dtype) -> P' x.(dbody) -> (forall x, P x -> p x -> f x = g x) ->
-  (forall x, P' x -> p' x -> f' x = g' x) ->
-  test_def p p' x ->
-  map_def f f' x = map_def g g' x.
-Proof.
-  intros. destruct x. unfold map_def. simpl.
-  unfold test_def in H1; simpl in H1. rewrite -> andb_and in H1. intuition.
-  rewrite !H // !H0 //; intuition auto.
-Qed.
-
-Lemma case_brs_forallb_map_spec {A B} {P : A -> Type} {p : A -> bool}
-      {l} {f g : A -> B} :
-  tCaseBrsProp P l ->
-  forallb (test_snd p) l ->
-  (forall x, P x -> p x -> f x = g x) ->
-  map (on_snd f) l = map (on_snd g) l.
-Proof.
-  intros.
-  eapply All_map_eq. red in X. apply forallb_All in H.
-  merge_All. eapply All_impl; eauto. simpl. intros. intuition.
-  eapply on_snd_test_spec; eauto.
-Qed.
-
-Lemma tfix_forallb_map_spec {A B} {P P' : A -> Prop} {p p'} {l} {f f' g g' : A -> B} :
-  tFixProp P P' l ->
-  forallb (test_def p p') l ->
-  (forall x, P x -> p x -> f x = g x) ->
-  (forall x, P' x -> p' x -> f' x = g' x) ->
-  map (map_def f f') l = map (map_def g g') l.
-Proof.
-  intros.
-  eapply All_map_eq; red in X. apply forallb_All in H.
-  merge_All. eapply All_impl; eauto. simpl; intros; intuition.
-  eapply map_def_test_spec; eauto.
-Qed.
-
-Ltac apply_spec :=
-  match goal with
-  | H : All _ _, H' : forallb _ _ = _ |- map _ _ = map _ _ =>
-    eapply (All_forallb_map_spec H H')
-  | H : All _ _, H' : forallb _ _ = _ |- forallb _ _ = _ =>
-    eapply (All_forallb_forallb_spec H H')
-  | H : tCaseBrsProp _ _, H' : forallb _ _ = _ |- map _ _ = map _ _ =>
-    eapply (case_brs_forallb_map_spec H H')
-  | H : All _ _, H' : is_true (forallb _ _) |- map _ _ = map _ _ =>
-    eapply (All_forallb_map_spec H H')
-  | H : All _ _, H' : is_true (forallb _ _) |- forallb _ _ = _ =>
-    eapply (All_forallb_forallb_spec H H')
-  | H : tCaseBrsProp _ _, H' : is_true (forallb _ _) |- map _ _ = map _ _ =>
-    eapply (case_brs_forallb_map_spec H H')
-  | H : tCaseBrsProp _ _ |- map _ _ = map _ _ =>
-    eapply (case_brs_map_spec H)
-  | H : tFixProp _ _ _, H' : forallb _ _ = _ |- map _ _ = map _ _ =>
-    eapply (tfix_forallb_map_spec H H')
-  | H : tFixProp _ _ _ |- map _ _ = map _ _ =>
-    eapply (tfix_map_spec H)
-  | H : All _ _ |- map _ _ = map _ _ =>
-    eapply (All_map_eq H)
-  | H : All _ _ |- map _ _ = _ =>
-    eapply (All_map_id H)
-  | H : All _ _ |- is_true (forallb _ _) =>
-    eapply (All_forallb _ _ H); clear H
-  end.
-
-
+(* todo move *)
 Ltac close_All :=
   match goal with
   | H : Forall _ _ |- Forall _ _ => apply (Forall_impl H); clear H; simpl
@@ -813,6 +361,7 @@ Proof.
   induction l in x |- *; simpl; simp list_size. lia.
   rewrite IHl. simpl. lia.
 Qed.
+
 Lemma mkApps_eq_head {x l} : mkApps x l = x -> l = [].
 Proof.
   assert (WF := _ : WellFounded (MR lt size)).
@@ -921,14 +470,6 @@ Proof.
 Qed.
 Close Scope string_scope.
 
-Lemma firstn_add {A} x y (args : list A) : firstn (x + y) args = firstn x args ++ firstn y (skipn x args).
-Proof.
-  induction x in y, args |- *. simpl. reflexivity.
-  simpl. destruct args. simpl.
-  now rewrite firstn_nil.
-  rewrite IHx. now rewrite app_comm_cons.
-Qed.
-
 Lemma decompose_app_rec_inv' f l hd args :
   decompose_app_rec f l = (hd, args) ->
   ∑ n, ~~ isApp hd /\ l = skipn n args /\ f = mkApps hd (firstn n args).
@@ -1009,10 +550,3 @@ Ltac solve_discr :=
         | [ H : is_true (application_atom (mkApps _ _)) |- _ ] =>
           destruct (application_atom_mkApps H); subst; try discriminate
         end)).
-
-(** Use a coercion for this common projection of the global context. *)
-Definition fst_ctx : global_env_ext -> global_env := fst.
-Coercion fst_ctx : global_env_ext >-> global_env.
-
-Definition empty_ext (Σ : global_env) : global_env_ext
-  := (Σ, Monomorphic_ctx ContextSet.empty).
