template-coq/theories/utils/MCString.v
@@ -1,5 +1,19 @@
 From Coq Require Import String.
+From MetaCoq.Template Require Import MCCompare.
 
+Local Open Scope string_scope.
+
+Definition string_of_list_aux {A} (f : A -> string) (sep : string) (l : list A) : string :=
+  let fix aux l :=
+      match l return string with
+      | nil => ""
+      | cons a nil => f a
+      | cons a l => f a ++ sep ++ aux l
+      end
+  in aux l.
+
+Definition string_of_list {A} (f : A -> string) (l : list A) : string :=
+  "[" ++ string_of_list_aux f "," l ++ "]".
 
 Definition string_of_nat n : string :=
   match n with
@@ -57,3 +71,16 @@ Definition string_of_nat n : string :=
   end.
 
 Hint Resolve String.string_dec : eq_dec.
+
+
+Definition eq_string s s' :=
+  match string_compare s s' with
+  | Eq => true
+  | _ => false
+  end.
+
+Lemma eq_string_refl x : is_true (eq_string x x).
+Proof.
+  unfold eq_string.
+  now rewrite (proj2 (string_compare_eq x x) eq_refl).
+Qed.
