erasure/theories/SafeTemplateErasure.v
@@ -20,10 +20,10 @@ Local Open Scope string_scope.
 
 Program Definition erase_template_program_check (p : Ast.program)
   : EnvCheck (EAst.global_context * EAst.term) :=
-  let Σ := List.rev (trans_global (AstUtils.empty_ext p.1)).1 in
+  let Σ := List.rev (trans_global (Ast.empty_ext p.1)).1 in
   G <- check_wf_env Σ ;;
-  Σ' <- wrap_error (PCUICAstUtils.empty_ext Σ) "erasure of the global context" (erase_global Σ _) ;;
-  t <- wrap_error (PCUICAstUtils.empty_ext Σ) ("During erasure of " ++ string_of_term (trans p.2)) (erase (empty_ext Σ) _ nil _ (trans p.2));;
+  Σ' <- wrap_error (empty_ext Σ) "erasure of the global context" (erase_global Σ _) ;;
+  t <- wrap_error (empty_ext Σ) ("During erasure of " ++ string_of_term (trans p.2)) (erase (empty_ext Σ) _ nil _ (trans p.2));;
   ret (Monad:=envcheck_monad) (Σ', t).
 
 Next Obligation.
@@ -131,10 +131,10 @@ Program Fixpoint check_wf_env_only_univs (Σ : global_env)
 
 Program Definition erase_template_program (p : Ast.program)
   : EnvCheck (EAst.global_context * EAst.term) :=
-  let Σ := List.rev (trans_global (AstUtils.empty_ext p.1)).1 in
+  let Σ := List.rev (trans_global (Ast.empty_ext p.1)).1 in
   G <- check_wf_env_only_univs Σ ;;
-  Σ' <- wrap_error (PCUICAstUtils.empty_ext Σ) "erasure of the global context" (SafeErasureFunction.erase_global Σ _) ;;
-  t <- wrap_error (PCUICAstUtils.empty_ext Σ) ("During erasure of " ++ string_of_term (trans p.2)) (SafeErasureFunction.erase (empty_ext Σ) _ nil (trans p.2) _);;
+  Σ' <- wrap_error (empty_ext Σ) "erasure of the global context" (SafeErasureFunction.erase_global Σ _) ;;
+  t <- wrap_error (empty_ext Σ) ("During erasure of " ++ string_of_term (trans p.2)) (SafeErasureFunction.erase (empty_ext Σ) _ nil (trans p.2) _);;
   ret (Monad:=envcheck_monad) (Σ', t).
 
 Next Obligation.
@@ -158,7 +158,7 @@ Program Definition erase_and_print_template_program_check {cf : checker_flags} (
   let p := fix_program_universes p in
   match erase_template_program_check p return string + string with
   | CorrectDecl (Σ', t) =>
-    inl ("Environment is well-formed and " ++ Pretty.print_term (AstUtils.empty_ext p.1) [] true p.2 ++
+    inl ("Environment is well-formed and " ++ Pretty.print_term (Ast.empty_ext p.1) [] true p.2 ++
          " erases to: " ++ nl ++ EPretty.print_term Σ' [] true false t)
   | EnvError Σ' (AlreadyDeclared id) =>
     inr ("Already declared: " ++ id)
@@ -172,7 +172,7 @@ Program Definition erase_and_print_template_program {cf : checker_flags} (p : As
   let p := fix_program_universes p in
   match erase_template_program p return string + string with
   | CorrectDecl (Σ', t) =>
-    inl ("Environment is well-formed and " ++ Pretty.print_term (AstUtils.empty_ext p.1) [] true p.2 ++
+    inl ("Environment is well-formed and " ++ Pretty.print_term (Ast.empty_ext p.1) [] true p.2 ++
          " erases to: " ++ nl ++ EPretty.print_term Σ' [] true false t)
   | EnvError Σ' (AlreadyDeclared id) =>
     inr ("Already declared: " ++ id)
