pcuic/theories/PCUICWeakening.v
@@ -572,7 +572,8 @@ Hint Rewrite lift_it_mkProd_or_LetIn : lift.
 Lemma to_extended_list_lift n k c :
   to_extended_list (lift_context n k c) = to_extended_list c.
 Proof.
-  unfold to_extended_list, to_extended_list_k. generalize 0. generalize (nil term) at 1 2.
+  unfold to_extended_list, to_extended_list_k. generalize 0.
+  unf_term. generalize (nil term) at 1 2.
   induction c in n, k |- *; simpl; intros. 1: reflexivity.
   rewrite -> lift_context_snoc0. unfold snoc. simpl.
   destruct a. destruct decl_body.
@@ -585,7 +586,7 @@ Lemma to_extended_list_map_lift:
   forall (n k : nat) (c : context), to_extended_list c = map (lift n (#|c| + k)) (to_extended_list c).
 Proof.
   intros n k c.
-  pose proof (to_extended_list_lift_above c).
+  pose proof (to_extended_list_lift_above c). unf_term.
   symmetry. solve_all.
   destruct H as [x' [-> Hx]]. simpl.
   destruct (leb_spec_Set (#|c| + k) x').
@@ -859,7 +860,7 @@ Proof.
   intros ity eq.
   pose proof (lift_destArity [] ity n k) as H; cbn in H. rewrite H; clear H.
   destruct destArity as [[ctx s] | ]; [|reflexivity]. simpl. f_equal.
-  rewrite lift_it_mkProd_or_LetIn; cbn. f_equal. f_equal.
+  rewrite lift_it_mkProd_or_LetIn; cbn. unf_term. f_equal. f_equal.
   - destruct idecl; reflexivity.
   - rewrite lift_mkApps; cbn; f_equal. rewrite map_app. f_equal.
     + rewrite !map_map lift_context_length; apply map_ext. clear.
